Arithmetization/ISigmaOne/HFS.lean
@@ -2,4 +2,5 @@ import Arithmetization.ISigmaOne.HFS.Basic
 import Arithmetization.ISigmaOne.HFS.Seq
 import Arithmetization.ISigmaOne.HFS.PRF
 import Arithmetization.ISigmaOne.HFS.Fixpoint
+import Arithmetization.ISigmaOne.HFS.Vec
 import Arithmetization.ISigmaOne.HFS.Supplemental
